keccak based proof

Generated/erc20shim/ERC20Shim/mapping_index_access_mapping_address_uint256_of_address_user.lean
@@ -14,17 +14,19 @@ open Clear EVMState Ast Expr Stmt FunctionDefinition State Interpreter ExecLemma
 
 abbrev AddressMap := Finmap (λ _ : Address ↦ UInt256)
 
+set_option linter.setOption false
+set_option pp.coercions false
+
 def A_mapping_index_access_mapping_address_uint256_of_address (dataSlot : Identifier) (slot key : Literal) (s₀ s₉ : State) : Prop :=
   let account := Address.ofUInt256 key
   ∀ {map : AddressMap}, account ∈ map →
-  ∃ address,
-  s₀.evm.keccak_map.lookup [ ↑account , slot ] = some address ∧
-  some (s₀.evm.sload address) = map.lookup account →
+  ∀ address,
+  s₀.evm.keccak_map.lookup [ ↑account , slot ] = some address →
   s₉ = s₀ ⟦ dataSlot ↦ address ⟧
 
   -- account ∈ erc20.balances →
   -- ∃ address, s₀.evm.keccak_map.lookup [ ↑account,  ERC20Private.balances ] = some address →
-  -- s₉ = s₀ ⟦ dataSlot ↦ address ⟧ 
+  -- s₉ = s₀ ⟦ dataSlot ↦ address ⟧
 
   -- let s₁ := s₀ 🇪⟦ s₀.evm.mstore 0x00 (Address.ofUInt256 key) ⟧
   -- let s₂ := s₁ 🇪⟦ s₁.evm.mstore 0x20 slot ⟧
@@ -62,7 +64,7 @@ def A_mapping_index_access_mapping_address_uint256_of_address (dataSlot : Identi
 
 -- lemma lookup_addr_fail {dataSlot : Identifier} {slot key : Literal} {s₀ s₉ : State}
 --   : A_mapping_index_access_mapping_address_uint256_of_address dataSlot slot key s₀ s₉ →
---     s₉.evm.hash_collision = true → 
+--     s₉.evm.hash_collision = true →
 --     s₉[dataSlot]!! = 0 := by
 --   intro r_addr h
 --   rcases s₀ with ⟨evm, varstore⟩ | _ | _ <;> [simp only; aesop_spec; aesop_spec]
@@ -71,20 +73,20 @@ def A_mapping_index_access_mapping_address_uint256_of_address (dataSlot : Identi
 
 --   unfold A_mapping_index_access_mapping_address_uint256_of_address at r_addr
 --   simp at r_addr
-  
+
 --   sorry
 
 -- lemma lookup_addr_ok {dataSlot : Identifier} {slot key : Literal} {s₀ s₉ : State}
 --   : A_mapping_index_access_mapping_address_uint256_of_address dataSlot slot key s₀ s₉ →
---     s₉.evm.hash_collision = false → 
+--     s₉.evm.hash_collision = false →
 --     ∃ addr, s₉[dataSlot]!! = addr := by
 --   intro r_addr
 --   sorry
 
   -- unfold A_mapping_index_access_mapping_address_uint256_of_address at r_addr
   -- simp at r_addr
-  
-  
+
+
   -- unfold setEvm at r_addr
   -- simp at r_addr
   -- generalize prep_def
@@ -97,7 +99,7 @@ def A_mapping_index_access_mapping_address_uint256_of_address (dataSlot : Identi
   --   use 0
   --   sorry
   -- | some a => sorry
-  
+
 -- Helper reifications
 lemma shift_eq_size : Fin.shiftLeft (n := UInt256.size) 1 160 = Address.size := by
   constructor
@@ -107,39 +109,48 @@ lemma EVMAddrSize' {s : State} : (s, [Fin.shiftLeft 1 160]) = (s, [Address.size.
   exact shift_eq_size
 
 lemma mapping_index_access_mapping_address_uint256_of_address_abs_of_concrete {s₀ s₉ : State} {dataSlot slot key} :
-  CollidingSpec (mapping_index_access_mapping_address_uint256_of_address_concrete_of_code.1 dataSlot slot key) s₀ s₉ →
-  CollidingSpec (A_mapping_index_access_mapping_address_uint256_of_address dataSlot slot key) s₀ s₉ := by
+  Spec (mapping_index_access_mapping_address_uint256_of_address_concrete_of_code.1 dataSlot slot key) s₀ s₉ →
+  Spec (A_mapping_index_access_mapping_address_uint256_of_address dataSlot slot key) s₀ s₉ := by
   unfold mapping_index_access_mapping_address_uint256_of_address_concrete_of_code A_mapping_index_access_mapping_address_uint256_of_address
   rcases s₀ with ⟨evm, varstore⟩ | _ | _ <;> [simp only; aesop_spec; aesop_spec]
-  apply collision_spec_eq'
-  
-  intro noCollision hasFuel
-  
+  apply spec_eq
+
+  intro hasFuel
   clr_funargs
 
   rw [ EVMSub', EVMShl', EVMAddrSize' ]; simp
   rw [ Address.and_size_eq_ofUInt256 ]
   rw [ multifill_cons, multifill_nil ]
   simp
-  
+
   clr_varstore
 
   generalize acconut_def : Address.ofUInt256 key = account
-  
-  intro prog erc20 account_mem_balances
-  
+
+  intro prog erc20 account_mem_balances address hasAddress
+
   rcases (Finmap.mem_iff.mp account_mem_balances) with ⟨bal, h_bal⟩
-  sorry
+
   -- use address
   -- intro h_lookup
-  -- generalize prep_def : (mstore evm 0 ↑↑account).mstore 32 slot = state_prep
+  generalize prep_def : (mstore evm 0 ↑↑account).mstore 32 slot = state_prep
 
-  -- have : Option.isSome $ state_prep.keccak256 0 64 := by
-  --   unfold keccak256
-  --   unfold mkInterval
-  --   unfold MachineState.lookupMemory
-  --   unfold_let
- 
+  have : Option.isSome $ state_prep.keccak256 0 64 := by
+    unfold keccak256
+    rw [← prep_def, interval'_eq_interval 2 two_ne_zero (by norm_cast)]
+
+
+    rw [ mstore_mstore_of_ne, interval_of_mstore_eq_val_cons
+       , mstore_mstore_of_ne, zero_add, interval_of_mstore_eq_val_cons
+       , interval_of_0_eq_nil
+       ]
+    unfold_let
+    rw [hasAddress]
+
+
+  sorry
+-- mkInterval (mstore evm x v) x = v :: (mkInterval evm (x + 32))
+  -- mkInterval evm n n = []
   --   rw [ ← prep_def ]
   --   unfold mstore updateMemory
   --   sorry
